setup execution example in parallel_for_omp_exec.v

concurrency/openmp_sem/parallel_for.c
@@ -1,0 +1,21 @@
+// gcc parallel_for.c -o parallel_for -fopenmp -lpthread
+// OMP_NESTED=TRUE OMP_NUM_THREADS=6 ./parallel_for
+#include <omp.h>
+#include <stdio.h>
+
+int main() {
+    
+    int count = 0;
+    #pragma omp parallel num_threads(3)
+    {
+        #pragma omp for reduction (+:count)
+        for (int i=0; i<6; i+=1) {
+            count += 1;
+
+            int *ptr1=&count;
+            int *ptr2=&i;
+        }
+    }
+    //printf("count=%d\n", count);
+    return 0;
+}
