concurrency/openmp_sem/notations.v
@@ -1,7 +1,7 @@
 From Coq Require Import String ZArith.
 From compcert Require Import Clightdefs AST.
 From compcert Require Export -(notations) lib.Maps.
-
+From stdpp Require Import base tactics.
 Local Open Scope string_scope.
 Local Open Scope clight_scope.
 (* same as in Clightdefs, just redefine notation *)
@@ -15,3 +15,40 @@ Notation "$$ s" := (ltac:(ClightNotations.ident_of_string s))
 Notation "a ! b" := (PTree.get b a) (at level 1).
 Notation "a !!!! b" := (PMap.get b a) (at level 1).
 
+Ltac unfold_mbind_in_hyp := 
+    lazymatch goal with
+    | [ H : context[@mbind _ ?instance _ _ _] |- _] => unfold mbind in H; unfold instance in H
+    end.
+
+(* destruct the first pattern matching in hyp *)
+Ltac destruct_match :=
+    lazymatch goal with
+    | [ _ : context[if (decide (?x = ?y)) then _ else _] |- _] => destruct (decide (x = y)) as [->|]; try done
+    | [ _ : context[match (match ?x with _ => _ end) with _ => _ end] |- _] => destruct x eqn:?; try done
+    | [ _ : context[match ?x with _ => _ end] |- _] => destruct x eqn:?; try done
+    end.
+
+Ltac destruct_match_in H :=
+    lazymatch type of H with
+    | context[if (decide (?x = ?y)) then _ else _] => destruct (decide (x = y)) as [->|]; try done
+    | context[match (match ?x with _ => _ end) with _ => _ end] => destruct x eqn:?; try done
+    | context[match ?x with _ => _ end] => destruct x eqn:?; try done
+    end.
+
+Ltac destruct_match_no_eqn :=
+    lazymatch goal with
+    | [ _ : context[if (decide (?x = ?y)) then _ else _] |- _] => destruct (decide (x = y)) as [->|]; try done
+    | [ _ : context[match (match ?x with _ => _ end) with _ => _ end] |- _] => destruct x; try done
+    | [ _ : context[match ?x with _ => _ end] |- _] => destruct x; try done
+    end.
+
+Ltac destruct_match_no_eqn_in H :=
+    lazymatch type of H with
+    | context[if (decide (?x = ?y)) then _ else _] => destruct (decide (x = y)) as [->|]; try done
+    | context[match (match ?x with _ => _ end) with _ => _ end] => destruct x; try done
+    | context[match ?x with _ => _ end] => destruct x; try done
+    end.
+
+Tactic Notation "destruct_match!" := destruct_match_no_eqn.
+Tactic Notation "destruct_match" "in" ident(H) := destruct_match_in H.
+Tactic Notation "destruct_match!" "in" ident(H) := destruct_match_no_eqn_in H.
