concurrency/openmp_sem/parallel_for_omp_exec.v
@@ -1,0 +1,143 @@
+From compcert Require Import Values Clight Memory Ctypes AST Globalenvs Integers.
+From compcert Require Import -(notations) Maps.
+Import PTree.
+From VST.concurrency.openmp_sem Require Import HybridMachineSig HybridMachine threadPool clight_fun notations team_dyn Clight_evsem.
+Import HybridMachineSig.
+Import ThreadPool. Import OrdinalPool.
+From VST.concurrency.openmp_sem Require Import parallel_for_omp.
+From stdpp Require Import base tactics.
+From Coq Require Import Relations.Relation_Operators Numbers.BinNums.
+From mathcomp.ssreflect Require Import ssreflect.
+From Hammer Require Import Tactics.
+
+
+Definition ge := Clight.globalenv prog.
+Instance Sem : Semantics := @Sem ge.
+Instance OrdinalThreadPoolInst: ThreadPool := OrdinalPool.OrdinalThreadPool.
+Instance OpenMP_semantics : MachineSig := @DryHybridMachineSig _ _.
+Definition OpenMP_steps := @Ostep_refl_trans_closure _ _.
+
+Definition init_mem : option mem := Genv.init_mem prog.
+
+(* OpenMP_semantics.(init_mach) is memory_semantics.initial_core *)
+(*  OpenMP_semantics.(init_mach): option res → mem → thread_pool → mem → val → list val → Prop *)
+
+Definition init_Ostate (os:@Ostate ge OrdinalPool.OrdinalThreadPool) : Prop :=
+    ∃ m b q U,
+    Genv.init_mem prog = Some m ∧
+    Genv.find_symbol (Genv.globalenv prog) (prog_main prog) = Some b ∧
+    OpenMP_semantics.(init_mach) None m q m (Vptr b Ptrofs.zero) nil ∧
+    os = ((U, [], q, team_init 0), m).
+
+Ltac evar_same_type_as i j :=
+        match type of j with | ?Tj => evar (i: Tj) end.
+Tactic Notation "evar!" ident(i) "type" "of" ident(j) := evar_same_type_as i j.
+
+Lemma exist_modus_ponens {A:Type} (P Q:A->Prop):
+    (∀ x, P x -> Q x) ->
+    (∃ a, P a) ->
+    ∃ a, Q a.
+Proof.
+    intros.
+    destruct H0 as [a Ha].
+    exists a.
+    apply H.
+    apply Ha.
+Qed.
+
+Instance DilMem : DiluteMem := HybridCoarseMachine.DilMem.
+Arguments DilMem: simpl never.
+Arguments diluteMem : simpl never.
+
+Instance scheduler : Scheduler := HybridCoarseMachine.scheduler.
+
+Ltac inv' H :=
+    let H' := fresh in
+    inversion H as [H']; clear H; rename H' into H; symmetry in H.
+
+Theorem parallel_for_exec :
+    ∀ os1, init_Ostate os1 ->
+    os1.1.1.1.1 = [0] ->
+    ∃ os2, OpenMP_steps os1 os2.
+Proof.
+    intros os1 H HU.
+    (* get initial state *)
+    unfold init_Ostate in H.
+    destruct H as (m&b&tp&U&Hm&Hb&Hinit&Hos).
+    simpl in Hinit. unfold DryHybridMachine.init_mach in Hinit.
+    destruct Hinit as (c&Hc&Hq). simpl in Hc. destruct_match! in Hc. clear e.
+    destruct Hc as [Hc _]. destruct_match in Hc. rename Heqo into Hf.
+    inv' Hc.
+    remember (team_init 0) as ttree.
+
+    destruct os1 as ((((U1 & tr1) & tp1) & ttree1) & m1) eqn: Hos1.
+    simpl in HU. inversion Hos. 
+    
+    (* take steps *)
+    eexists.
+
+    (** take 1st step *)
+    (* build assumptions for threadStep*)
+    assert (cnt0: ThreadPool.containsThread tp 0).
+    { subst. done. }
+    assert (Hcompat0: mem_compatible tp m).
+    { admit. }
+
+    pose tid:nat:=0.
+    pose U2:=@yield scheduler U.
+    evar (ev:list openmp_sem.event_semantics.mem_event).
+    pose tr2:=(seq.cat tr1 (List.map (fun mev => Events.internal 0 mev) ev))%list.
+    evar (le: env).
+    pose tp2:= ThreadPool.updThread cnt0
+    (Krun
+       (Clight_core.State f_main (fn_body f_main) Kstop le
+          (set _ptr1 Vundef
+             (set _ptr2 Vundef (set _t'3 Vundef (set _t'2 Vundef (set _t'1 Vundef (PTree.empty val))))))))
+    (openmp_sem.permissions.getCurPerm m, (ThreadPool.getThreadR cnt0).2).
+
+    pose ttree2:=ttree1.
+    (* evar! m2 type of m. *)
+    apply (rt1n_trans Ostate Ostep _ (U2, tr2, tp2, ttree, diluteMem m)).
+    { 
+        (* build preconditions for evstep *)
+        (* compute f *)
+        rewrite /Genv.find_symbol /Genv.genv_symb in Hb.
+        unfold PTree.get in Hb.
+        simpl in Hb.
+        inv' Hb.
+        rewrite Hb /Genv.find_funct_ptr  /= in Hf.
+        inv' Hf.
+
+        (* compute m *)
+        (* rewrite /Genv.init_mem /prog /Clightdefs.mkprogram /= in Hm. *)
+        
+
+        (* take a threadStep *)
+        rewrite /Ostep /MachStep /=.
+        subst tr2. subst tr1.
+        subst U2.
+        eapply (thread_step 0 U tp tp2 m m ev [] ttree _ cnt0 Hcompat0).
+        rewrite /= /DryHybridMachine.threadStep.
+        eapply (step_dry(m:=m) cnt0 Hcompat0 _ c m m _ ev).
+        { cbn. admit. }
+        { econstructor; admit. }
+        { rewrite /= /getThreadC. subst tp; done. }
+        {
+            (* take ev_step *)
+            rewrite /openmp_sem.event_semantics.ev_step /=.
+            rewrite Hc.
+            rewrite Hf.
+            eapply evstep_internal_function.
+            { sauto. }
+            { unfold Coqlib.list_disjoint. intros. sauto. }
+            { repeat (constructor; sauto). }
+            {  admit. }
+            { sauto. }
+        }
+        reflexivity.
+    }
+
+    (** take 2nd step *)
+Admitted.
+
+    
